src/Bedrock/P256/JacobianAffine.v
@@ -1,0 +1,389 @@
+Require Import coqutil.Datatypes.List Coq.Lists.List.
+Require Import Bedrock.P256.Specs.
+
+Import Specs.NotationsCustomEntry Specs.coord Specs.point.
+Import Curves.Weierstrass.P256.
+
+Import bedrock2.Syntax bedrock2.NotationsCustomEntry
+LittleEndianList
+Crypto.Util.ZUtil.Modulo Zdiv ZArith BinInt
+BinInt BinNat Init.Byte
+PrimeFieldTheorems ModInv
+micromega.Lia
+coqutil.Byte
+Lists.List micromega.Lia
+Jacobian
+Coq.Strings.String Coq.Lists.List
+ProgramLogic WeakestPrecondition
+ProgramLogic.Coercions
+Word.Interface OfListWord Separation SeparationLogic
+letexists
+BasicC64Semantics
+ListIndexNotations
+SepAutoArray
+symmetry
+PeanoNat micromega.Lia
+Tactics
+UniquePose
+micromega.Lia Word.Properties.
+
+Import Zbool. (*compat 8.20*)
+Import ListIndexNotations.
+Local Open Scope list_index_scope.
+Local Open Scope Z_scope.
+Local Open Scope bool_scope.
+Local Open Scope string_scope.
+Local Open Scope list_scope.
+
+Local Notation "xs $@ a" := (map.of_list_word_at a xs)
+  (at level 10, format "xs $@ a").
+Local Notation "$ n" := (match word.of_Z n return word with w => w end) (at level 9, format "$ n").
+Local Notation "p .+ n" := (word.add p (word.of_Z n)) (at level 50, format "p .+ n", left associativity).
+Local Coercion F.to_Z : F >-> Z.
+
+
+Import Coq.micromega.Lia.
+Import coqutil.Tactics.Tactics.
+
+
+Definition fe_set_1 := func! (o) {
+  o0 = $1; o1 = $0xffffffff00000000; o2 = -$1; o3 = $0xfffffffe;
+  store(o, o0); store(o+$8, o1); store(o+$16, o2); store(o+$24, o3)
+}.
+
+Definition p256_point_add_affine_nz_nz_neq := func! (p_out, p_P, p_Q) ~> ok {
+  stackalloc 32 as z1z1;
+  stackalloc 32 as u2;
+  stackalloc 32 as h;
+  stackalloc 32 as s2;
+  stackalloc 32 as r;
+  stackalloc 32 as Hsqr;
+  stackalloc 32 as Hcub;
+
+  p256_coord_sqr(z1z1, p_P.+$32.+$32);
+  p256_coord_mul(u2, p_Q, z1z1);
+  p256_coord_sub(h, u2, p_P);
+  p256_coord_mul(s2, p_P.+$32.+$32, z1z1);
+  p256_coord_mul(p_out.+$32.+$32, h, p_P.+$32.+$32);
+  p256_coord_mul(s2, s2, p_Q.+$32);
+  p256_coord_sub(r, s2, p_P.+$32);
+  p256_coord_sqr(Hsqr, h);
+  p256_coord_sqr(p_out, r);
+  p256_coord_mul(Hcub, Hsqr, h);
+  p256_coord_mul(u2, p_P, Hsqr);
+
+  unpack! different_x = p256_coord_nonzero(Hcub);
+  unpack! different_y = p256_coord_nonzero(p_out);
+  unpack! ok = br_value_barrier(different_x | different_y);
+
+  p256_coord_sub(p_out, p_out, Hcub);
+  p256_coord_sub(p_out, p_out, u2);
+  p256_coord_sub(p_out, p_out, u2);
+  p256_coord_sub(h, u2, p_out);
+  p256_coord_mul(s2, Hcub, p_P.+$32);
+  p256_coord_mul(h, h, r);
+  p256_coord_sub(p_out.+$32, h, s2)
+}.
+
+Local Ltac length_tac_rewrites :=
+  repeat rewrite
+    ?length_coord, ?length_point,
+    ?app_length, ?firstn_length, ?skipn_length, ?length_le_split, ?length_nil,
+    ?Nat.min_l in *
+    by (trivial; lia).
+Local Ltac length_tac := repeat straightline_cleanup;length_tac_rewrites; trivial; lia.
+
+Local Ltac clear_nongoal_sephyps :=
+  repeat match reverse goal with
+  | H : (_ * _)%sep ?m |- _ =>
+      tryif match goal with |- context[m] => idtac end
+      then try rename H into Hm
+      else clear H; try clear m
+  | m : Interface.map.rep |- _ => clear m
+  end.
+
+Local Ltac clear_nonsymex_sephyps :=
+  tryif
+  match goal with
+  | |- Semantics.call _ _ _ _ _ _ => idtac
+  | |- cmd _ _ _ _ _ _ => idtac
+  | |- expr _ _ _ _ => idtac
+  | |- dexpr _ _ _ _ => idtac
+  | |- load _ _ _ _ => idtac
+  | |- store _ _ _ _ _ => idtac
+  | |- Memory.load _ _ _ = _ => idtac
+  end
+  then clear_nongoal_sephyps else idtac.
+
+Local Ltac symex_call := (straightline_call; ssplit; [ solve [
+      repeat match goal with
+      | |- True => exact I
+      | |- exists _, _ => letexists
+      | |- _ _ => ecancel_assumption
+      | |- _ => length_tac
+      end
+    ] ..  | repeat straightline_cleanup; straightline; repeat straightline_cleanup; clear_nonsymex_sephyps; repeat straightline]).
+
+Lemma p256_point_add_affine_nz_nz_neq_ok : program_logic_goal_for_function! p256_point_add_affine_nz_nz_neq.
+Proof.
+  cbv [spec_of_p256_point_add_affine_nz_nz_neq of_affine].
+  straightline; repeat straightline_cleanup.
+  destruct P as (((x1 & y1) & z1) & p1), (Jacobian.of_affine Q) as (((x2 & y2) & z2) & p2) eqn:HeqQ;
+    cbv [proj1_sig proj2_sig fst snd point.to_bytes] in * |-.
+  match goal with H : _ m |- context[m] => rename H into Hm end.
+
+  rewrite <-(firstn_skipn 32 out) in Hm.
+  rewrite <-(firstn_skipn 32 (skipn _ out)) in Hm.
+  progress repeat seprewrite_in_by Array.sep_eq_of_list_word_at_app Hm length_tac.
+
+  repeat straightline. clear_nonsymex_sephyps.
+  repeat seprewrite_in_by Array.array1_iff_eq_of_list_word_at Hm ltac:(Lia.lia).
+  progress change (Z.of_nat 32) with 32 in *.
+
+  symex_call.
+  symex_call.
+  symex_call.
+  symex_call.
+  symex_call.
+  symex_call.
+  symex_call.
+  symex_call.
+  symex_call.
+  symex_call.
+  symex_call.
+  symex_call.
+  symex_call.
+  symex_call.
+  symex_call.
+  symex_call.
+  symex_call.
+  symex_call.
+  symex_call.
+  symex_call.
+  symex_call.
+  clear_nongoal_sephyps.
+
+  (* stackdealloc *)
+  progress repeat seprewrite_in_by (symmetry! @Array.array1_iff_eq_of_list_word_at) Hm ltac:(rewrite ?length_coord; Lia.lia).
+  progress repeat match type of Hm with context [Array.array ptsto _ _ (coord.to_bytes ?x)] =>
+    unique pose proof (length_coord x) end.
+  repeat straightline. clear_nongoal_sephyps.
+  progress repeat seprewrite_in_by (@Array.array1_iff_eq_of_list_word_at) Hm ltac:(rewrite ?length_coord; Lia.lia).
+  length_tac_rewrites.
+
+  (* postcondition *)
+
+  cbv [proj1_sig proj2_sig fst snd point.to_bytes ].
+  seprewrite_in_by (Array.list_word_at_app_of_adjacent_eq(p_Q)(p_Q.+32)) Hm ltac:(length_tac_rewrites; listZnWords).
+  seprewrite_in_by (Array.list_word_at_app_of_adjacent_eq(p_Q)(p_Q.+32.+32)) Hm ltac:(length_tac_rewrites; listZnWords).
+  seprewrite_in_by (Array.list_word_at_app_of_adjacent_eq(p_P)(p_P.+32)) Hm ltac:(length_tac_rewrites; listZnWords).
+  seprewrite_in_by (Array.list_word_at_app_of_adjacent_eq(p_P)(p_P.+32.+32)) Hm ltac:(length_tac_rewrites; listZnWords).
+  seprewrite_in_by (Array.list_word_at_app_of_adjacent_eq(p_out)(p_out.+32)) Hm ltac:(length_tac_rewrites; listZnWords).
+  seprewrite_in_by (Array.list_word_at_app_of_adjacent_eq(p_out)(p_out.+32.+32)) Hm ltac:(length_tac_rewrites; listZnWords).
+  eexists; ssplit.
+  { use_sep_assumption. cancel. repeat ecancel_step. Morphisms.f_equiv. }
+  { length_tac. }
+  clear Hm.
+
+  intros.
+  cbv [affine_point.iszero] in *.
+  destruct Q as ([[]|[]]&?) in HeqQ, H59; [|contradiction]; apply (f_equal (@proj1_sig _ _)) in HeqQ;
+      cbv [of_affine Jacobian.of_affine Jacobian.of_affine_impl fst snd Jacobian.eq proj1_sig] in HeqQ; Prod.inversion_prod; subst.
+
+  case (Properties.word.eqb_spec x3 $0); subst x3; rewrite word.lor_0_iff; [right|left]; split; trivial.
+  { subst x x0.
+    rewrite !word.broadcast_0_iff in *.
+    rewrite !Bool.negb_false_iff, !F.eqb_eq in *.
+    cbv [of_affine Jacobian.of_affine fst snd Jacobian.eq Jacobian.iszero proj1_sig] in *.
+    case H60 as [Hx Hy].
+    case Decidable.dec; intros; try contradiction; split; [apply Hierarchy.one_neq_zero|].
+    rewrite Hierarchy.commutative in Hx.
+    rewrite <-!F.pow_succ_r in Hx, Hy; simpl N.succ in Hx, Hy.
+    rewrite F.pow_0_iff, Ring.sub_zero_iff in Hx, Hy by (lia||exact _).
+    rewrite ?F.pow_3_r, ?F.pow_2_r in Hx.
+    rewrite ?F.pow_3_r, ?F.pow_2_r in Hy.
+    split; Field.fsatz. }
+  { unshelve eexists ?[pfPneqQ].
+    { intros HX; cbv [Jacobian.eq Jacobian.iszero of_affine Jacobian.of_affine Jacobian.of_affine_impl proj1_sig fst snd] in H59, H60, HX.
+      destruct Decidable.dec in HX; try contradiction; case HX as (Hz&Hx&Hy).
+      apply H60. subst x x0.
+      rewrite !word.broadcast_0_iff in *.
+      rewrite !Bool.negb_false_iff, !F.eqb_eq.
+      rewrite ?F.pow_3_r, ?F.pow_2_r, ?Hx, ?Hy, ?(proj2 (Ring.sub_zero_iff _ _)); ssplit; Field.fsatz. }
+    cbv [Jacobian.add_inequal_nz_nz Jacobian.add_inequal_impl of_affine Jacobian.of_affine Jacobian.of_affine_impl proj1_sig fst snd point.to_bytes]; cbn [fst snd proj1_sig].
+    rewrite ?app_assoc, ?F.pow_3_r, ?F.pow_2_r; repeat (ring || f_equal). }
+Qed.
+
+
+Definition p256_point_add_affinenz_conditional_vartime_if_doubling := func! (p_out, p_P, p_Q, c) {
+  unpack! zeroP = p256_point_iszero(p_P);
+  unpack! nzQ = br_broadcast_nonzero(c);
+  zeroQ = ~nzQ;
+  stackalloc (3*32) as p_tmp;
+  unpack! ok = p256_point_add_affine_nz_nz_neq(p_tmp, p_P, p_Q);
+  unpack! ok = br_declassify(zeroP | zeroQ | ok);
+  stackalloc (3*32) as p_buf;
+  br_memset(p_buf, $0, $3*$32);
+  br_memcxor(p_buf, p_tmp,  $3*$32,     ~zeroP & ~zeroQ);
+  br_memcxor(p_buf, p_P,    $3*$32,     ~zeroP &  zeroQ);
+  br_memcxor(p_buf, p_Q,    $3*$32,      zeroP & ~zeroQ);
+  if !ok { p256_point_double(p_buf, p_P) };
+  br_memcpy(p_out, p_buf, $(3*32))
+}.
+
+From bedrock2Examples Require Import memcpy.
+
+Lemma p256_point_add_affinenz_conditional_vartime_if_doubling_ok : program_logic_goal_for_function! p256_point_add_affinenz_conditional_vartime_if_doubling.
+Proof.
+  cbv [spec_of_p256_point_add_affinenz_conditional_vartime_if_doubling].
+  repeat straightline.
+  match goal with H : _ m |- context[m] => rename H into Hm end.
+
+  straightline_call; repeat straightline. (*iszero*)
+  { letexists. ecancel_assumption. }
+  straightline_call; repeat straightline. (*broadcast*)
+  (* stackalloc *)
+  seprewrite_in_by (@Array.array1_iff_eq_of_list_word_at) Hm ltac:(lia).
+  straightline_call; ssplit. (*add*)
+  { ecancel_assumption. }
+  { rewrite length_point; lia. }
+  repeat straightline.
+  straightline_call; repeat straightline (* br_declassify *).
+  (* stackalloc *)
+  clear_nonsymex_sephyps.
+  seprewrite_in_by (@Array.array1_iff_eq_of_list_word_at) Hm ltac:(lia).
+  straightline_call; ssplit. (* memset *)
+  { ecancel_assumption. }
+  { ZnWords.ZnWords. }
+  repeat straightline.
+  straightline_call; repeat straightline; ssplit (* memcxor *).
+  { ecancel_assumption. }
+  { rewrite ?repeat_length; trivial. }
+  { rewrite H17, length_point; trivial. }
+  straightline_call; repeat straightline; ssplit (* memcxor *).
+  { ecancel_assumption. }
+  { rewrite ?repeat_length; trivial. }
+  { rewrite length_point; trivial. }
+  straightline_call; repeat straightline; ssplit (* memcxor *).
+  { ecancel_assumption. }
+  { rewrite ?repeat_length; trivial. }
+  { rewrite length_point; trivial. }
+  clear_nonsymex_sephyps.
+  progress rewrite ?word.unsigned_mul_nowrap, ?word.unsigned_of_Z_nowrap in * by ZnWords.ZnWords.
+
+assert (word__and_broadcast : forall a b, word.and (word.broadcast a) (word.broadcast b) = word.broadcast (andb a b)). {
+  clear; intros a b; case a, b; cbv [word.broadcast]; trivial.
+}
+
+  cbv [affine_point.iszero] in *; subst zeroQ.
+  subst x x0 x3.
+  cbn [Semantics.interp_op1] in *; rewrite ?word.not_broadcast, ?word__and_broadcast, ?Bool.negb_involutive in *.
+
+  letexists; ssplit; repeat straightline; subst v (* if ok *).
+  { straightline_call; repeat straightline; ssplit (* memcpy *).
+    { ecancel_assumption. }
+    { rewrite H10, length_point; trivial. }
+    { trivial. }
+    { clear; ZnWords.ZnWords. }
+    clear_nongoal_sephyps.
+    (* stackdealloc *)
+    progress repeat seprewrite_in_by (symmetry! (Array.array1_iff_eq_of_list_word_at a)) Hm ltac:(length_tac_rewrites; listZnWords).
+    progress repeat seprewrite_in_by (symmetry! (Array.array1_iff_eq_of_list_word_at a0)) Hm ltac:(length_tac_rewrites; listZnWords).
+    assert (Datatypes.length x6 = 96%nat) by (length_tac_rewrites; listZnWords).
+    assert (Datatypes.length x2 = 96%nat) by (length_tac_rewrites; listZnWords).
+    repeat straightline; clear_nongoal_sephyps.
+
+    rewrite <-word.unsigned_of_Z_0, !word.unsigned_inj_iff in H16 by exact _.
+    rewrite !word.lor_0_iff, !word.broadcast_0_iff in H16.
+    destruct (iszero P) eqn:HP in *; (destruct (word.eqb_spec c2 (word.of_Z 0)) as [|HQ] in *; [subst c2|]);
+      repeat (cbn [Z.eqb negb andb] in *; rewrite ?Z.eqb_refl in *; rewrite ?(proj2 (Z.eqb_neq _ _)) in * by ZnWords.ZnWords;
+        match goal with
+           | H : word.broadcast false = word.of_Z 0 -> _ |- _ => specialize (H eq_refl)
+           | H : word.broadcast true = word.of_Z (-1) -> _ |- _ => specialize (H eq_refl)
+           end); subst; rewrite ?Byte.map_xor_0_l in * by (rewrite ?length_point; ZnWords.ZnWords).
+    { (* 0 + 0 *)
+      apply Decidable.dec_bool, Jacobian.iszero_iff in HP.
+      eexists (exist _ (0,0,0)%F I); split.
+      { use_sep_assumption; cancel. reflexivity. }
+      rewrite Jacobian.eq_iff, HP; reflexivity. }
+    { (* 0 + Q *)
+      apply Decidable.dec_bool, Jacobian.iszero_iff in HP.
+      eexists; split. { ecancel_assumption. }
+      rewrite Jacobian.eq_iff, Jacobian.to_affine_add, HP.
+      symmetry.
+      eapply Hierarchy.left_identity. }
+    { (* P + 0 *)
+      eexists; split. { ecancel_assumption. } reflexivity. }
+    { (* nz + nz' *)
+      (* Decidable.dec_iff? *)
+      cbv [iszero] in HP, HQ; case Decidable.dec in HP; try congruence.
+      destruct (H18 ltac:(trivial) ltac:(intros HX; specialize (H11 HX); congruence)) as [ [_ (?&HE)] |]; [|intuition fail].
+      repeat straightline_cleanup.
+      eexists; split; [ecancel_assumption|].
+      rewrite Jacobian.eq_iff, Jacobian.to_affine_add, Jacobian.to_affine_add_inequal_nz_nz; trivial; [reflexivity|].
+      rewrite Jacobian.iszero_iff, Jacobian.to_affine_of_affine.
+      destruct Q as ([(?&?)|[]]&?); intuition idtac.
+    } }
+  { (* if !ok *)
+    rewrite <-word.unsigned_of_Z_0, word.unsigned_inj_iff in * by exact _.
+    rewrite !word.lor_0_iff, !word.broadcast_0_iff in *.
+    DestructHead.destruct_head' @and; subst.
+    rewrite ?word.not_broadcast, ?word__and_broadcast, ?Bool.negb_involutive, ?word.broadcast_0_iff, ?Z.eqb_neq, ?word.unsigned_of_Z_0 in *.
+
+    straightline_call; repeat straightline.
+    { split. { ecancel_assumption. } { length_tac. } }
+    straightline_call; repeat straightline; ssplit (* memcpy *).
+    { ecancel_assumption. }
+    { rewrite H10, length_point; trivial. }
+    { trivial. }
+    { clear; ZnWords.ZnWords. }
+    repeat straightline.
+    (* stackdealloc *)
+    clear_nongoal_sephyps.
+    progress repeat seprewrite_in_by (symmetry! (Array.array1_iff_eq_of_list_word_at a)) Hm ltac:(length_tac_rewrites; listZnWords).
+    progress repeat seprewrite_in_by (symmetry! (Array.array1_iff_eq_of_list_word_at a0)) Hm ltac:(length_tac_rewrites; listZnWords).
+    assert (Datatypes.length x6 = 96%nat) by (length_tac_rewrites; listZnWords).
+    assert (Datatypes.length ((to_bytes (Jacobian.double_minus_3 eq_refl P))) = 96%nat) by (length_tac_rewrites; listZnWords).
+    repeat straightline; clear_nongoal_sephyps.
+
+    eexists; ssplit. { ecancel_assumption. }
+    destruct (word.eqb_spec c2 (word.of_Z 0)); [subst; rewrite ?word.unsigned_of_Z_0 in *; contradiction|].
+    rewrite <-Jacobian.double_minus_3_eq_double.
+    rewrite Jacobian.eq_iff, Jacobian.to_affine_double, Jacobian.to_affine_add; Morphisms.f_equiv.
+    enough (Jacobian.eq P Q) as -> by reflexivity.
+
+    cbv [iszero] in *; case Decidable.dec in *; try congruence.
+    destruct (H18 ltac:(trivial) ltac:(intros HX; specialize (H11 HX); congruence)) as [ [? (?&HE)] |]; [congruence|intuition fail]. }
+Qed.
+
+
+Definition sc_halve := func!(y, x) {
+  unpack! m = br_value_barrier(-(load(x)&$1)); (* is x odd? *)
+  mh0 = $0x79dce5617e3192a8; mh1 = $0xde737d56d38bcf42; mh2 = $0x7fffffffffffffff; mh3 = $0x7fffffff80000000; (* minus one half modulo l *)
+  stackalloc 32 as mmh; (* maybe minus half *)
+  store(mmh, m&mh0); store(mmh+$8, m&mh1); store(mmh+$16, m&mh2); store(mmh+$24, m&mh3);
+  y0 = load(y); y1 = load(y+$8); y2 = load(y+$16); y3 = load(y+$24);
+  unpack! y0 = shrd_64(y0, y1, $1);
+  unpack! y1 = shrd_64(y1, y2, $1);
+  unpack! y2 = shrd_64(y2, y3, $1);
+  y3 = y3 >> $1;
+  store(y, y0); store(y+$8, y1); store(y+$16, y2); store(y+$24, y3);
+  sc_sub(y, y, mmh)
+}.
+
+Definition sc_sub := func!(out, x, y) {
+  unpack! x1, x2 = sbb64($0, load(x), load(y));
+  unpack! x3, x4 = sbb64(x2, load(x+$8), load(y+$8));
+  unpack! x5, x6 = sbb64(x4, load(x+$16), load(y+$16));
+  unpack! x7, x8 = sbb64(x6, load(x+$24), load(y+$24));
+  x9 = -x8;
+  unpack! x10, x11 = adc64($0, x1, x9 & $0xf3b9cac2fc632551);
+  unpack! x12, x13 = adc64(x11, x3, x9 & $0xbce6faada7179e84);
+  unpack! x14, x15 = adc64(x13, x5, x9);
+  unpack! x16, x17 = adc64(x15, x7, x9 << $32);
+  x17 = x17+$0;
+  store(out, x10);
+  store(out+$8, x12);
+  store(out+$16, x14);
+  store(out+$24, x16)
+}.
